@prefix laderr: <https://w3id.org/laderr#> .
@prefix dct: <http://purl.org/dc/terms/> .
@prefix mod: <https://w3id.org/mod#> .
@prefix owl: <http://www.w3.org/2002/07/owl#> .
@prefix rdf: <http://www.w3.org/1999/02/22-rdf-syntax-ns#> .
@prefix xml: <http://www.w3.org/XML/1998/namespace> .
@prefix xsd: <http://www.w3.org/2001/XMLSchema#> .
@prefix dcat: <http://www.w3.org/ns/dcat#> .
@prefix foaf: <http://xmlns.com/foaf/0.1/> .
@prefix rdfs: <http://www.w3.org/2000/01/rdf-schema#> .
@prefix skos: <http://www.w3.org/2004/02/skos/core#> .
@prefix vann: <http://purl.org/vocab/vann/> .
@base <https://w3id.org/laderr#> .

<https://w3id.org/laderr#> rdf:type owl:Ontology ;
                            dct:abstract """LaDeRR Vocabulary is an OWL-based ontology designed to formally define the core concepts and relationships of Language for Describing Risk and Resilience (LaDeRR). Grounded in the ResiliOnt ontology, LaDeRR enables machine-readable representations of resilience scenarios.

This vocabulary provides a structured semantic framework to represent key resilience elements, including entities, capabilities, vulnerabilities, threats, dispositions, controls, and resilience. It incorporates logical constraints and derivation rules to ensure semantic correctness and facilitate automated reasoning.

The LaDeRR Vocabulary is developed to support interoperability with domain-specific applications, enabling consistency in resilience assessments, decision support, and computational modeling. It is implemented in OWL 2 and follows best practices in ontology engineering to ensure extensibility and usability across various domains."""@en ;
                            dct:contributor <https://orcid.org/0000-0001-9247-6150> ,
                                            <https://orcid.org/0000-0002-3452-553X> ,
                                            <https://orcid.org/0000-0003-0481-9745> ;
                            dct:creator <https://orcid.org/0000-0003-2736-7817> ;
                            dct:description "OWL vocabulary for LaDeRR (Language for Describing Risk and Resilience), a domain-specific language for modeling risk and resilience scenarios. This vocabulary provides a canonical RDF-based serialization of the language, enabling publication, data exchange, and computational processing. It also serves as a schema to validate and support LaDeRR instances represented as RDF graphs."@en ;
                            dct:identifier "https://w3id.org/laderr" ;
                            dct:issued "2025-01-14"^^xsd:date ;
                            dct:language "en"^^xsd:language ;
                            dct:license <https://www.apache.org/licenses/LICENSE-2.0> ;
                            dct:modified "2025-03-30"^^xsd:date ;
                            dct:publisher <https://ugent-businessinformatics.github.io/> ,
                                          <https://www.flandersmake.be/> ,
                                          <https://www.utwente.nl/en/eemcs/scs/> ;
                            dct:title "LaDeRR Vocabulary"@en ;
                            vann:preferredNamespacePrefix "laderr" ;
                            vann:preferredNamespaceUri "https://w3id.org/laderr#"^^xsd:anyURI ;
                            owl:versionInfo "Revised LaDeRR vocabulary with disjointness axioms, equivalent class definitions, renamed individuals and properties, and improved resilience constraints. Vocabulary structure aligned with OWL 2 best practices and updated semantics."@en ;
                            dcat:keyword "DSL"@en ,
                                         "incident"@en ,
                                         "laderr"@en ,
                                         "resilience"@en ,
                                         "risk"@en ;
                            dcat:landingPage <https://w3id.org/laderr/git> ;
                            dcat:version "0.8.3" ;
                            foaf:homepage <https://w3id.org/laderr> ;
                            foaf:logo <https://raw.githubusercontent.com/pedropaulofb/laderr/refs/heads/main/resources/logo_laderr.png> ;
                            mod:repository <https://w3id.org/laderr/git> .

#################################################################
#    Annotation properties
#################################################################

###  http://purl.org/dc/terms/contributor
dct:contributor rdf:type owl:AnnotationProperty .


###  http://purl.org/dc/terms/creator
dct:creator rdf:type owl:AnnotationProperty .


###  http://purl.org/dc/terms/description
dct:description rdf:type owl:AnnotationProperty .


###  http://purl.org/dc/terms/identifier
dct:identifier rdf:type owl:AnnotationProperty .


###  http://purl.org/dc/terms/issued
dct:issued rdf:type owl:AnnotationProperty .


###  http://purl.org/dc/terms/language
dct:language rdf:type owl:AnnotationProperty .


###  http://purl.org/dc/terms/license
dct:license rdf:type owl:AnnotationProperty .


###  http://purl.org/dc/terms/modified
dct:modified rdf:type owl:AnnotationProperty .


###  http://purl.org/dc/terms/publisher
dct:publisher rdf:type owl:AnnotationProperty .


###  http://purl.org/dc/terms/title
dct:title rdf:type owl:AnnotationProperty .


###  http://purl.org/vocab/vann/preferredNamespacePrefix
vann:preferredNamespacePrefix rdf:type owl:AnnotationProperty .


###  http://purl.org/vocab/vann/preferredNamespaceUri
vann:preferredNamespaceUri rdf:type owl:AnnotationProperty .


###  http://www.w3.org/2002/07/owl#versionInfo
owl:versionInfo rdf:type owl:AnnotationProperty .


###  http://www.w3.org/2004/02/skos/core#example
skos:example rdf:type owl:AnnotationProperty .


###  http://www.w3.org/2004/02/skos/core#note
skos:note rdf:type owl:AnnotationProperty .


###  http://www.w3.org/ns/dcat#keyword
dcat:keyword rdf:type owl:AnnotationProperty .


###  http://www.w3.org/ns/dcat#landingPage
dcat:landingPage rdf:type owl:AnnotationProperty .


###  http://www.w3.org/ns/dcat#version
dcat:version rdf:type owl:AnnotationProperty .


###  http://xmlns.com/foaf/0.1/homepage
foaf:homepage rdf:type owl:AnnotationProperty .


###  http://xmlns.com/foaf/0.1/logo
foaf:logo rdf:type owl:AnnotationProperty .


###  http://xmlns.com/foaf/0.1/mbox
foaf:mbox rdf:type owl:AnnotationProperty .


###  http://xmlns.com/foaf/0.1/member
foaf:member rdf:type owl:AnnotationProperty .


###  http://xmlns.com/foaf/0.1/name
foaf:name rdf:type owl:AnnotationProperty .


###  https://w3id.org/mod#repository
mod:repository rdf:type owl:AnnotationProperty .


#################################################################
#    Datatypes
#################################################################

###  http://www.w3.org/2001/XMLSchema#date
xsd:date rdf:type rdfs:Datatype .


#################################################################
#    Object Properties
#################################################################

###  https://w3id.org/laderr#canDamage
laderr:canDamage rdf:type owl:ObjectProperty ;
                 rdfs:subPropertyOf laderr:positiveDamage ;
                 rdfs:domain laderr:Threat ;
                 rdfs:range laderr:Asset ;
                 rdfs:comment "Indicates that a Threat can cause value loss to an Asset in an operational Scenario."@en ;
                 rdfs:isDefinedBy <https://w3id.org/laderr> ;
                 rdfs:label "canDamage"@en .


###  https://w3id.org/laderr#cannotDamage
laderr:cannotDamage rdf:type owl:ObjectProperty ;
                    rdfs:subPropertyOf laderr:negativeDamage ;
                    rdfs:domain laderr:Threat ;
                    rdfs:range laderr:Asset ;
                    rdfs:comment "Indicates that a Threat cannot cause value loss to an Asset in an operational Scenario."@en ;
                    rdfs:isDefinedBy <https://w3id.org/laderr> ;
                    rdfs:label "cannotDamage"@en .


###  https://w3id.org/laderr#capabilities
laderr:capabilities rdf:type owl:ObjectProperty ;
                    rdfs:domain laderr:Entity ;
                    rdfs:range laderr:Capability ;
                    rdfs:comment "Associates an Entity with the Capabilities it possesses."@en ;
                    rdfs:isDefinedBy <https://w3id.org/laderr> ;
                    rdfs:label "capabilities"@en .


###  https://w3id.org/laderr#components
laderr:components rdf:type owl:ObjectProperty ;
                  owl:inverseOf laderr:scenarios ;
                  rdfs:domain laderr:Scenario ;
                  rdfs:range laderr:ScenarioComponent ;
                  rdfs:comment "Links a Scenario to the ScenarioComponents it is composed of, such as Entities, Dispositions, and Resilience constructs."@en ;
                  rdfs:isDefinedBy <https://w3id.org/laderr> ;
                  rdfs:label "components"@en .


###  https://w3id.org/laderr#constructs
laderr:constructs rdf:type owl:ObjectProperty ;
                  rdfs:domain laderr:Specification ;
                  rdfs:range laderr:Construct ;
                  rdfs:comment "Links a Specification to the Constructs it defines, including Scenarios and their components."@en ;
                  rdfs:isDefinedBy <https://w3id.org/laderr> ;
                  rdfs:label "constructs"@en .


###  https://w3id.org/laderr#damaged
laderr:damaged rdf:type owl:ObjectProperty ;
               rdfs:subPropertyOf laderr:positiveDamage ;
               rdfs:domain laderr:Threat ;
               rdfs:range laderr:Asset ;
               rdfs:comment "Indicates that a Threat caused value loss to an Asset in an incident Scenario."@en ;
               rdfs:isDefinedBy <https://w3id.org/laderr> ;
               rdfs:label "damaged"@en .


###  https://w3id.org/laderr#disables
laderr:disables rdf:type owl:ObjectProperty ,
                         owl:IrreflexiveProperty ;
                rdfs:domain laderr:Capability ;
                rdfs:range laderr:Disposition ;
                rdfs:comment "Indicates that an enabled Capability changes the state of a Disposition (either a Capability or Vulnerability) to disabled, preventing it from being realized. This implies the disabler must be enabled and the target must have been previously enabled."@en ;
                skos:example "A water cooling system's capability of keeping temperatures below critical thresholds disables the 'overheat' vulnerability in a server rack."@en ;
                rdfs:isDefinedBy <https://w3id.org/laderr> ;
                rdfs:label "disables"@en .


###  https://w3id.org/laderr#exploits
laderr:exploits rdf:type owl:ObjectProperty ;
                rdfs:domain laderr:Capability ;
                rdfs:range laderr:Vulnerability ;
                rdfs:comment "Defines the relationship where a Capability exploits a Vulnerability, meaning that when both are enabled, the Capability can trigger an adverse event through the Vulnerability."@en ;
                rdfs:isDefinedBy <https://w3id.org/laderr> ;
                rdfs:label "exploits"@en .


###  https://w3id.org/laderr#exposes
laderr:exposes rdf:type owl:ObjectProperty ;
               rdfs:domain laderr:Vulnerability ;
               rdfs:range laderr:Capability ;
               rdfs:comment "Defines that a Vulnerability exposes a Capability, making it susceptible to threats."@en ;
               rdfs:isDefinedBy <https://w3id.org/laderr> ;
               rdfs:label "exposes"@en .


###  https://w3id.org/laderr#inhibits
laderr:inhibits rdf:type owl:ObjectProperty ;
                rdfs:domain laderr:Control ;
                rdfs:range laderr:Threat ;
                rdfs:comment "An Entity inhibits another if it has a Capability that disables a Vulnerability, while the inhibited Entity has a Capability that exploits the same Vulnerability."@en ;
                rdfs:isDefinedBy <https://w3id.org/laderr> ;
                rdfs:label "inhibits"@en .


###  https://w3id.org/laderr#negativeDamage
laderr:negativeDamage rdf:type owl:ObjectProperty ;
                      rdfs:domain laderr:Threat ;
                      rdfs:range laderr:Asset ;
                      rdfs:comment "Superclass for relationships that indicate a negative occurrence of damage. Encompasses relations where a Threat either cannot cause or did not cause damage to an Asset. I.e., depending on the scenario’s situation, it is realized as laderr:cannotDamage (operational) or laderr:notDamaged (incident)"@en ;
                      rdfs:isDefinedBy <https://w3id.org/laderr> ;
                      rdfs:label "negativeDamage"@en .


###  https://w3id.org/laderr#notDamaged
laderr:notDamaged rdf:type owl:ObjectProperty ;
                  rdfs:subPropertyOf laderr:negativeDamage ;
                  rdfs:domain laderr:Threat ;
                  rdfs:range laderr:Asset ;
                  rdfs:comment "Indicates that a Threat did not cause loss of value to an Asset in a Scenario with situation 'incident'."@en ;
                  rdfs:isDefinedBy <https://w3id.org/laderr> ;
                  rdfs:label "notDamaged"@en .


###  https://w3id.org/laderr#positiveDamage
laderr:positiveDamage rdf:type owl:ObjectProperty ;
                      rdfs:domain laderr:Threat ;
                      rdfs:range laderr:Asset ;
                      rdfs:comment "Superclass for relationships that indicate a positive occurrence of damage. Encompasses relations where a Threat either can cause or has caused damage to an Asset. I.e., depending on the scenario’s situation, it is realized as laderr:canDamage (operational) or laderr:damaged (incident)"@en ;
                      rdfs:isDefinedBy <https://w3id.org/laderr> ;
                      rdfs:label "positiveDamage"@en .


###  https://w3id.org/laderr#preserves
laderr:preserves rdf:type owl:ObjectProperty ;
                 rdfs:domain laderr:Resilience ;
                 rdfs:range laderr:Capability ;
                 rdfs:comment "Indicates that a Resilience maintains the functionality and value of a Capability within a Scenario."@en ;
                 rdfs:isDefinedBy <https://w3id.org/laderr> ;
                 rdfs:label "preserves"@en .


###  https://w3id.org/laderr#preservesAgainst
laderr:preservesAgainst rdf:type owl:ObjectProperty ;
                        rdfs:domain laderr:Resilience ;
                        rdfs:range laderr:Capability ;
                        rdfs:comment "Indicates that a Resilience maintains a Capability’s function despite the presence of a Threat's Capability that could exploit a Vulnerability."@en ;
                        rdfs:isDefinedBy <https://w3id.org/laderr> ;
                        rdfs:label "preservesAgainst"@en .


###  https://w3id.org/laderr#preservesDespite
laderr:preservesDespite rdf:type owl:ObjectProperty ;
                        rdfs:domain laderr:Resilience ;
                        rdfs:range laderr:Vulnerability ;
                        rdfs:comment "Indicates that a Resilience ensures a Capability remains functional despite an existing Vulnerability exposing it."@en ;
                        rdfs:isDefinedBy <https://w3id.org/laderr> ;
                        rdfs:label "preservesDespite"@en .


###  https://w3id.org/laderr#protects
laderr:protects rdf:type owl:ObjectProperty ;
                rdfs:domain laderr:Control ;
                rdfs:range laderr:Asset ;
                rdfs:comment "Represents a relationship where an Entity prevents harm to another Entity by possessing a Capability that disables a Vulnerability that Threats might exploit."@en ;
                rdfs:isDefinedBy <https://w3id.org/laderr> ;
                rdfs:label "protects"@en .


###  https://w3id.org/laderr#resiliences
laderr:resiliences rdf:type owl:ObjectProperty ;
                   rdfs:domain laderr:Asset ;
                   rdfs:range laderr:Resilience ;
                   rdfs:comment "Links an Asset to its associated Resiliences."@en ;
                   rdfs:isDefinedBy <https://w3id.org/laderr> ;
                   rdfs:label "resiliences"@en .


###  https://w3id.org/laderr#scenarios
laderr:scenarios rdf:type owl:ObjectProperty ;
                 rdfs:domain laderr:ScenarioComponent ;
                 rdfs:range laderr:Scenario ;
                 rdfs:comment "Links a ScenarioComponent to the Scenarios they are part of."@en ;
                 rdfs:isDefinedBy <https://w3id.org/laderr> ;
                 rdfs:label "scenarios"@en .


###  https://w3id.org/laderr#situation
laderr:situation rdf:type owl:ObjectProperty ;
                 rdfs:domain laderr:Scenario ;
                 rdfs:range laderr:ScenarioSituation ;
                 rdfs:comment "Associates a Scenario with a ScenarioSituation describing whether it is operational or an incident."@en ;
                 rdfs:isDefinedBy <https://w3id.org/laderr> ;
                 rdfs:label "situation"@en .


###  https://w3id.org/laderr#state
laderr:state rdf:type owl:ObjectProperty ;
             rdfs:domain laderr:Disposition ;
             rdfs:range laderr:DispositionState ;
             rdfs:comment "Defines whether a Disposition (Capability or Vulnerability) is active (enabled) or inactive (disabled). The state determines its eligibility for, e.g., exploitation and disabling."@en ;
             rdfs:isDefinedBy <https://w3id.org/laderr> ;
             rdfs:label "state"@en .


###  https://w3id.org/laderr#status
laderr:status rdf:type owl:ObjectProperty ;
              rdfs:domain laderr:Scenario ;
              rdfs:range laderr:ScenarioStatus ;
              rdfs:comment "Defines the resilience status of a Scenario: whether it cannot be damaged by threats (resilient) or not (vulnerable)."@en ;
              rdfs:isDefinedBy <https://w3id.org/laderr> ;
              rdfs:label "status"@en .


###  https://w3id.org/laderr#sustains
laderr:sustains rdf:type owl:ObjectProperty ;
                rdfs:domain laderr:Capability ;
                rdfs:range laderr:Resilience ;
                rdfs:comment "Represents the relationship between a Capability and a Resilience where the Capability enables the conditions necessary for the Resilience to exist."@en ;
                rdfs:isDefinedBy <https://w3id.org/laderr> ;
                rdfs:label "sustains"@en .


###  https://w3id.org/laderr#threatens
laderr:threatens rdf:type owl:ObjectProperty ;
                 rdfs:domain laderr:Threat ;
                 rdfs:range laderr:Asset ;
                 rdfs:comment "Indicates that a Threat poses risk to an Asset by potentially exploiting its Vulnerabilities."@en ;
                 rdfs:isDefinedBy <https://w3id.org/laderr> ;
                 rdfs:label "threatens"@en .


###  https://w3id.org/laderr#vulnerabilities
laderr:vulnerabilities rdf:type owl:ObjectProperty ;
                       rdfs:domain laderr:Entity ;
                       rdfs:range laderr:Vulnerability ;
                       rdfs:comment "Associates an Entity with its Vulnerabilities, which may expose it to threats."@en ;
                       rdfs:isDefinedBy <https://w3id.org/laderr> ;
                       rdfs:label "vulnerabilities"@en .


#################################################################
#    Data properties
#################################################################

###  https://w3id.org/laderr#baseURI
laderr:baseURI rdf:type owl:DatatypeProperty ;
               rdfs:range xsd:anyURI ;
               rdfs:comment "Defines the base URI of a LaDeRR Specification."@en ;
               rdfs:isDefinedBy <https://w3id.org/laderr> ;
               rdfs:label "baseURI"@en .


###  https://w3id.org/laderr#createdBy
laderr:createdBy rdf:type owl:DatatypeProperty ;
                 rdfs:range rdfs:Literal ;
                 rdfs:comment "Indicates the creator of a LaDeRR Specification."@en ;
                 rdfs:isDefinedBy <https://w3id.org/laderr> ;
                 rdfs:label "createdBy"@en .


###  https://w3id.org/laderr#createdOn
laderr:createdOn rdf:type owl:DatatypeProperty ;
                 rdfs:range xsd:dateTime ;
                 rdfs:comment "Records the date and time when a LaDeRR Specification was created."@en ;
                 rdfs:isDefinedBy <https://w3id.org/laderr> ;
                 rdfs:label "createdOn"@en .


###  https://w3id.org/laderr#description
laderr:description rdf:type owl:DatatypeProperty ;
                   rdfs:range rdfs:Literal ;
                   rdfs:comment "Human-readable explanation of a Construct or Specification."@en ;
                   rdfs:isDefinedBy <https://w3id.org/laderr> ;
                   rdfs:label "description"@en .


###  https://w3id.org/laderr#modifiedOn
laderr:modifiedOn rdf:type owl:DatatypeProperty ;
                  rdfs:range xsd:dateTime ;
                  rdfs:comment "Records the date and time when a LaDeRR Specification was last modified."@en ;
                  rdfs:isDefinedBy <https://w3id.org/laderr> ;
                  rdfs:label "modifiedOn"@en .


###  https://w3id.org/laderr#title
laderr:title rdf:type owl:DatatypeProperty ;
             rdfs:range rdfs:Literal ;
             rdfs:comment "The title assigned to a LaDeRR Specification."@en ;
             rdfs:isDefinedBy <https://w3id.org/laderr> ;
             rdfs:label "title"@en .


###  https://w3id.org/laderr#version
laderr:version rdf:type owl:DatatypeProperty ;
               rdfs:range xsd:string ;
               rdfs:comment "Specifies the version of a LaDeRR Specification."@en ;
               rdfs:isDefinedBy <https://w3id.org/laderr> ;
               rdfs:label "version"@en .


#################################################################
#    Classes
#################################################################

###  http://xmlns.com/foaf/0.1/Organization
foaf:Organization rdf:type owl:Class .


###  https://w3id.org/laderr#Asset
laderr:Asset rdf:type owl:Class ;
             rdfs:subClassOf laderr:Entity ;
             rdfs:comment "An Asset represents an entity that has value and is subject to potential risks and threats."@en ;
             rdfs:isDefinedBy <https://w3id.org/laderr> ;
             rdfs:label "Asset"@en ;
             skos:example "A museum's ancient manuscript collection is an Asset because it holds historical and cultural value that can be lost."@en ;
             skos:note "Corresponds to the concept of Object at Risk in ResiliOnt."@en .


###  https://w3id.org/laderr#Capability
laderr:Capability rdf:type owl:Class ;
                  rdfs:subClassOf laderr:Disposition ;
                  rdfs:comment "A Capability is a disposition that enables an Entity to perform specific functions."@en ;
                  rdfs:isDefinedBy <https://w3id.org/laderr> ;
                  rdfs:label "Capability"@en ;
                  skos:example "A drone's night-vision camera is a Capability enabling surveillance in low-light rescue operations."@en ;
                  skos:note "Corresponds to the concept of Capability in ResiliOnt."@en .


###  https://w3id.org/laderr#Construct
laderr:Construct rdf:type owl:Class ;
                 owl:equivalentClass [ rdf:type owl:Class ;
                                       owl:unionOf ( laderr:Scenario
                                                     laderr:ScenarioComponent
                                                   )
                                     ] ;
                 rdfs:subClassOf [ rdf:type owl:Restriction ;
                                   owl:onProperty laderr:description ;
                                   owl:maxQualifiedCardinality "1"^^xsd:nonNegativeInteger ;
                                   owl:onDataRange xsd:string
                                 ] ;
                 rdfs:comment "An abstract class encompassing both Scenarios and ScenarioComponents. I.e., any instantiable construct expressible in a LaDeRR specification."@en ;
                 rdfs:isDefinedBy <https://w3id.org/laderr> ;
                 rdfs:label "Construct"@en .


###  https://w3id.org/laderr#Control
laderr:Control rdf:type owl:Class ;
               rdfs:subClassOf laderr:Entity ;
               rdfs:comment "A Control is an Entity that protects Assets by inhibiting threats (e.g., through disabling vulnerabilities)."@en ;
               rdfs:isDefinedBy <https://w3id.org/laderr> ;
               rdfs:label "Control"@en ;
               skos:example "A fire suppression system in a data center acts as a Control that inhibits fire-related threats and protects the servers."@en ;
               skos:note "Corresponds to the concept of Risk Inhibitor in ResiliOnt."@en .


###  https://w3id.org/laderr#Disposition
laderr:Disposition rdf:type owl:Class ;
                   owl:equivalentClass [ rdf:type owl:Class ;
                                         owl:unionOf ( laderr:Capability
                                                       laderr:Vulnerability
                                                     )
                                       ] ,
                                       [ rdf:type owl:Restriction ;
                                         owl:onProperty laderr:state ;
                                         owl:qualifiedCardinality "1"^^xsd:nonNegativeInteger ;
                                         owl:onClass laderr:DispositionState
                                       ] ;
                   rdfs:subClassOf laderr:ScenarioComponent ;
                   rdfs:comment "A Disposition is a potential of an Entity to exhibit certain behaviors or effects under specific conditions. It must be enabled in a scenario to exert influence and may be disabled by another Capability."@en ;
                   rdfs:isDefinedBy <https://w3id.org/laderr> ;
                   rdfs:label "Disposition"@en ;
                   skos:note "Corresponds to the concept of Disposition in ResiliOnt."@en .


###  https://w3id.org/laderr#DispositionState
laderr:DispositionState rdf:type owl:Class ;
                        owl:equivalentClass [ rdf:type owl:Class ;
                                              owl:oneOf ( laderr:disabled
                                                          laderr:enabled
                                                        )
                                            ] ;
                        rdfs:comment "Represents the state of a Disposition, which can be either ENABLED or DISABLED, determining whether it can be realized in a given scenario."@en ;
                        rdfs:isDefinedBy <https://w3id.org/laderr> ;
                        rdfs:label "DispositionState"@en ;
                        skos:example "During a system check, a sensor’s 'motion detection' feature might be in the DISABLED state to avoid false alarms."@en .


###  https://w3id.org/laderr#Entity
laderr:Entity rdf:type owl:Class ;
              owl:equivalentClass [ rdf:type owl:Class ;
                                    owl:unionOf ( laderr:Asset
                                                  laderr:Control
                                                  laderr:Threat
                                                )
                                  ] ;
              rdfs:subClassOf laderr:ScenarioComponent ,
                              [ rdf:type owl:Restriction ;
                                owl:onProperty laderr:capabilities ;
                                owl:someValuesFrom laderr:Capability
                              ] ;
              rdfs:comment "An Entity is a core participant in a Scenario, encompassing Assets, Threats, and Controls. Entities typically possess Capabilities and may have Vulnerabilities. They can protect, threaten, or inhibit others, depending on how their internal Dispositions are enabled. These interactions are derived from the interplay between their capabilities and vulnerabilities."@en ;
              rdfs:isDefinedBy <https://w3id.org/laderr> ;
              rdfs:label "Entity"@en ;
              skos:note "Corresponds to the concept of Value Object in ResiliOnt."@en .


###  https://w3id.org/laderr#Resilience
laderr:Resilience rdf:type owl:Class ;
                  owl:equivalentClass [ rdf:type owl:Restriction ;
                                        owl:onProperty laderr:preserves ;
                                        owl:someValuesFrom laderr:Capability
                                      ] ,
                                      [ rdf:type owl:Restriction ;
                                        owl:onProperty laderr:preservesAgainst ;
                                        owl:someValuesFrom laderr:Capability
                                      ] ,
                                      [ rdf:type owl:Restriction ;
                                        owl:onProperty laderr:preservesDespite ;
                                        owl:someValuesFrom laderr:Vulnerability
                                      ] ;
                  rdfs:subClassOf laderr:ScenarioComponent ;
                  rdfs:comment "Resilience maintains the function of Capabilities despite the presence of Vulnerabilities and threats that could exploit them, thereby contributing to the preservation of asset value within a Scenario. It emerges when an Entity possesses a Capability that disables a Vulnerability exposing another Capability, while another Entity has a Capability that could exploit that same Vulnerability."@en ;
                  rdfs:isDefinedBy <https://w3id.org/laderr> ;
                  rdfs:label "Resilience"@en ;
                  skos:example "A zebra herd maintains coordinated movement through its navigation Capability, which is preserved against predator threats and despite heat exhaustion vulnerabilities."@en ;
                  skos:note "Corresponds to the concept of Resilience in ResiliOnt."@en .


###  https://w3id.org/laderr#Scenario
laderr:Scenario rdf:type owl:Class ;
                rdfs:subClassOf laderr:Construct ,
                                [ rdf:type owl:Restriction ;
                                  owl:onProperty laderr:components ;
                                  owl:someValuesFrom laderr:ScenarioComponent
                                ] ,
                                [ rdf:type owl:Restriction ;
                                  owl:onProperty laderr:situation ;
                                  owl:qualifiedCardinality "1"^^xsd:nonNegativeInteger ;
                                  owl:onClass laderr:ScenarioSituation
                                ] ,
                                [ rdf:type owl:Restriction ;
                                  owl:onProperty laderr:status ;
                                  owl:qualifiedCardinality "1"^^xsd:nonNegativeInteger ;
                                  owl:onClass laderr:ScenarioStatus
                                ] ;
                owl:disjointWith laderr:ScenarioComponent ;
                rdfs:comment "Represents a present or past situation (operational or incident, respectively) in which Entities and their Dispositions interact, allowing the evaluation of resilience conditions."@en ;
                rdfs:isDefinedBy <https://w3id.org/laderr> ;
                rdfs:label "Scenario"@en ;
                skos:example "The 'Heatwave Response' scenario models an operational situation in which entities like the Zebra Herd and Meerkat Sentinels act through enabled capabilities to prevent threats from causing damage, demonstrating a resilient condition."@en .


###  https://w3id.org/laderr#ScenarioComponent
laderr:ScenarioComponent rdf:type owl:Class ;
                         owl:equivalentClass [ rdf:type owl:Class ;
                                               owl:unionOf ( laderr:Disposition
                                                             laderr:Entity
                                                             laderr:Resilience
                                                           )
                                             ] ;
                         rdfs:subClassOf laderr:Construct ;
                         rdfs:comment "A base construct in the LaDeRR vocabulary, representing fundamental elements such as entities, their dispositions, and resilience concepts."@en ;
                         rdfs:isDefinedBy <https://w3id.org/laderr> ;
                         rdfs:label "ScenarioComponent"@en .


###  https://w3id.org/laderr#ScenarioSituation
laderr:ScenarioSituation rdf:type owl:Class ;
                         owl:equivalentClass [ rdf:type owl:Class ;
                                               owl:oneOf ( laderr:incident
                                                           laderr:operational
                                                         )
                                             ] ;
                         rdfs:comment "An enumeration defining the nature of a scenario as either 'operational' or 'incident', describing its temporal context."@en ;
                         rdfs:isDefinedBy <https://w3id.org/laderr> ;
                         rdfs:label "ScenarioSituation"@en .


###  https://w3id.org/laderr#ScenarioStatus
laderr:ScenarioStatus rdf:type owl:Class ;
                      owl:equivalentClass [ rdf:type owl:Class ;
                                            owl:oneOf ( laderr:resilient
                                                        laderr:vulnerable
                                                      )
                                          ] ;
                      rdfs:comment "Represents the resilience status of a scenario, which can be either 'vulnerable' or 'resilient'."@en ;
                      rdfs:isDefinedBy <https://w3id.org/laderr> ;
                      rdfs:label "ScenarioStatus"@en .


###  https://w3id.org/laderr#Specification
laderr:Specification rdf:type owl:Class ;
                     rdfs:subClassOf [ rdf:type owl:Restriction ;
                                       owl:onProperty laderr:createdBy ;
                                       owl:someValuesFrom xsd:string
                                     ] ,
                                     [ rdf:type owl:Restriction ;
                                       owl:onProperty laderr:baseURI ;
                                       owl:qualifiedCardinality "1"^^xsd:nonNegativeInteger ;
                                       owl:onDataRange xsd:anyURI
                                     ] ,
                                     [ rdf:type owl:Restriction ;
                                       owl:onProperty laderr:createdOn ;
                                       owl:qualifiedCardinality "1"^^xsd:nonNegativeInteger ;
                                       owl:onDataRange xsd:dateTime
                                     ] ,
                                     [ rdf:type owl:Restriction ;
                                       owl:onProperty laderr:title ;
                                       owl:qualifiedCardinality "1"^^xsd:nonNegativeInteger ;
                                       owl:onDataRange xsd:string
                                     ] ,
                                     [ rdf:type owl:Restriction ;
                                       owl:onProperty laderr:description ;
                                       owl:maxQualifiedCardinality "1"^^xsd:nonNegativeInteger ;
                                       owl:onDataRange xsd:string
                                     ] ,
                                     [ rdf:type owl:Restriction ;
                                       owl:onProperty laderr:modifiedOn ;
                                       owl:maxQualifiedCardinality "1"^^xsd:nonNegativeInteger ;
                                       owl:onDataRange xsd:dateTime
                                     ] ,
                                     [ rdf:type owl:Restriction ;
                                       owl:onProperty laderr:version ;
                                       owl:maxQualifiedCardinality "1"^^xsd:nonNegativeInteger ;
                                       owl:onDataRange xsd:string
                                     ] ;
                     rdfs:comment "A structured document that defines one or more resilience scenarios, including constructs such as assets, threats, controls, and their interactions in specific operational or incident situations."@en ;
                     rdfs:isDefinedBy <https://w3id.org/laderr> ;
                     rdfs:label "Specification"@en ;
                     skos:example "The 'Savannah Animal Survival Resilience Model' specification defines a structured model with scenarios like 'Dry Season Survival' and 'Heatwave Response', including constructs such as threats, capabilities, vulnerabilities, and resiliences for ecological analysis."@en .


###  https://w3id.org/laderr#Threat
laderr:Threat rdf:type owl:Class ;
              owl:equivalentClass [ rdf:type owl:Restriction ;
                                    owl:onProperty laderr:threatens ;
                                    owl:someValuesFrom laderr:Asset
                                  ] ;
              rdfs:subClassOf laderr:Entity ;
              rdfs:comment "A Threat is an entity that can potentially cause harm to an Asset through its threat capabilities, by potentially exploiting the latter's Vulnerabilities."@en ;
              rdfs:isDefinedBy <https://w3id.org/laderr> ;
              rdfs:label "Threat"@en ;
              skos:example "A ransomware attack targeting hospital records is a Threat that endangers critical health information systems."@en ;
              skos:note "Corresponds to the concept of Threat Object in ResiliOnt."@en .


###  https://w3id.org/laderr#Vulnerability
laderr:Vulnerability rdf:type owl:Class ;
                     owl:equivalentClass [ rdf:type owl:Restriction ;
                                           owl:onProperty laderr:exposes ;
                                           owl:someValuesFrom laderr:Capability
                                         ] ;
                     rdfs:subClassOf laderr:Disposition ;
                     rdfs:comment "A disposition of an Entity that may be exploited by Threats, potentially leading to harm."@en ;
                     rdfs:isDefinedBy <https://w3id.org/laderr> ;
                     rdfs:label "Vulnerability"@en ;
                     skos:example "Outdated software in a system is a Vulnerability that exposes it to cyberattacks."@en ;
                     skos:note "Corresponds to the concept of Vulnerability in ResiliOnt."@en .


#################################################################
#    Individuals
#################################################################

###  https://ugent-businessinformatics.github.io/
<https://ugent-businessinformatics.github.io/> rdf:type owl:NamedIndividual ,
                                                        foaf:Organization ;
                                               foaf:homepage "https://ugent-businessinformatics.github.io/"^^xsd:anyURI ;
                                               foaf:member <https://orcid.org/0000-0001-9247-6150> ,
                                                           <https://orcid.org/0000-0003-0481-9745> ,
                                                           <https://orcid.org/0000-0003-2736-7817> ;
                                               foaf:name "UGent Business Informatics, Ghent University, Belgium" .


###  https://w3id.org/laderr#disabled
laderr:disabled rdf:type owl:NamedIndividual ,
                         laderr:DispositionState ;
                owl:differentFrom laderr:enabled ;
                rdfs:comment "Represents a DispositionState where a Capability or Vulnerability is inactive and cannot influence the system. A disabled Disposition cannot exert its effect until it is re-enabled."@en ;
                skos:example "A system’s temperature alarm is 'disabled' during maintenance, preventing it from influencing calculations."@en ;
                rdfs:isDefinedBy <https://w3id.org/laderr> ;
                rdfs:label "disabled"@en .


###  https://w3id.org/laderr#enabled
laderr:enabled rdf:type owl:NamedIndividual ,
                        laderr:DispositionState ;
               rdfs:comment "Represents a DispositionState where a Capability or Vulnerability is active and can influence the system. An enabled Capability can, e.g., sustain a resilience, while an enabled Vulnerability can be exploited by threats."@en ;
               skos:example "A drone's surveillance Capability is 'enabled' during a mission, allowing it to sustain communication."@en ;
               rdfs:isDefinedBy <https://w3id.org/laderr> ;
               rdfs:label "enabled"@en .


###  https://w3id.org/laderr#incident
laderr:incident rdf:type owl:NamedIndividual ,
                         laderr:ScenarioSituation ;
                owl:differentFrom laderr:operational ;
                rdfs:comment "Represents a scenario that has already occurred."@en ;
                rdfs:isDefinedBy <https://w3id.org/laderr> ;
                rdfs:label "incident"@en .


###  https://w3id.org/laderr#operational
laderr:operational rdf:type owl:NamedIndividual ,
                            laderr:ScenarioSituation ;
                   rdfs:comment "A scenario situation representing the system's current functioning, with or without threats and resiliences."@en ;
                   rdfs:isDefinedBy <https://w3id.org/laderr> ;
                   rdfs:label "operational"@en .


###  https://w3id.org/laderr#resilient
laderr:resilient rdf:type owl:NamedIndividual ,
                          laderr:ScenarioStatus ;
                 owl:differentFrom laderr:vulnerable ;
                 rdfs:comment "A scenario type where resiliences are sufficient to prevent threats from causing damage."@en ;
                 rdfs:isDefinedBy <https://w3id.org/laderr> ;
                 rdfs:label "resilient"@en .


###  https://w3id.org/laderr#vulnerable
laderr:vulnerable rdf:type owl:NamedIndividual ,
                           laderr:ScenarioStatus ;
                  rdfs:comment "A scenario type where the system lacks resilience, meaning threats successfully exploit vulnerabilities, leading to damage or loss."@en ;
                  rdfs:isDefinedBy <https://w3id.org/laderr> ;
                  rdfs:label "vulnerable"@en .


###  https://www.flandersmake.be/
<https://www.flandersmake.be/> rdf:type owl:NamedIndividual ,
                                        foaf:Organization ;
                               foaf:homepage "https://www.flandersmake.be/"^^xsd:anyURI ;
                               foaf:member <https://orcid.org/0000-0001-9247-6150> ,
                                           <https://orcid.org/0000-0003-0481-9745> ,
                                           <https://orcid.org/0000-0003-2736-7817> ;
                               foaf:name "Flanders Make, Belgium" .


###  https://www.utwente.nl/en/eemcs/scs/
<https://www.utwente.nl/en/eemcs/scs/> rdf:type owl:NamedIndividual ,
                                                foaf:Organization ;
                                       foaf:homepage "https://www.utwente.nl/en/eemcs/scs/"^^xsd:anyURI ;
                                       foaf:member <https://orcid.org/0000-0002-3452-553X> ,
                                                   <https://orcid.org/0000-0003-2736-7817> ;
                                       foaf:name "Semantics, Cybersecurity & Services (SCS), University of Twente, the Netherlands" .


#################################################################
#    Annotations
#################################################################

<https://orcid.org/0000-0001-9247-6150> foaf:name "Geert Poels" .


<https://orcid.org/0000-0002-3452-553X> foaf:name "Giancarlo Guizzardi" .


<https://orcid.org/0000-0003-0481-9745> foaf:name "Frederik Gailly" .


<https://orcid.org/0000-0003-2736-7817> foaf:mbox "pedropaulofb@gmail.com" ;
                                        foaf:name "Pedro Paulo Favato Barcelos" .


<https://w3id.org/laderr/git> rdfs:comment "Repository for the LaDeRR DSL."@en .


<https://w3id.org/laderr/ttl> rdfs:comment "TTL serialization of the LaDeRR-Vocabulary."@en .


#################################################################
#    General axioms
#################################################################

[ rdf:type owl:AllDisjointClasses ;
  owl:members ( laderr:Construct
                laderr:DispositionState
                laderr:ScenarioSituation
                laderr:ScenarioStatus
                laderr:Specification
              )
] .


[ rdf:type owl:AllDisjointClasses ;
  owl:members ( laderr:Disposition
                laderr:Entity
                laderr:Resilience
              )
] .
